lib/DataStructures/BtreeModel.i.dfy
@@ -1845,727 +1845,727 @@ abstract module BtreeModel {
     assert keys == Unzip(kvlist).0;
   }
 
-  predicate ValidBoundariesForSeqInner(nkeys: int, boundaries: seq<nat>)
-  {
-    && 1 < |boundaries|
-    && boundaries[0] == 0
-    && Last(boundaries) == nkeys
-    && Integer_Order.IsStrictlySorted(boundaries)
-  }
-
-  lemma ValidBoundariesForSeqBounds(nkeys: int, boundaries: seq<nat>)
-    ensures ValidBoundariesForSeqInner(nkeys, boundaries) ==>
-    && (forall i :: 0 <= i < |boundaries|-1 ==> boundaries[i] < nkeys)
-    && (forall i :: 1 <= i < |boundaries| ==> 0 < boundaries[i])
-  {
-    if ValidBoundariesForSeqInner(nkeys, boundaries) {
-      forall i | 0 <= i < |boundaries|-1
-        ensures boundaries[i] < nkeys
-      {
-        Integer_Order.IsStrictlySortedImpliesLt(boundaries, i, |boundaries|-1);
-      }
-      forall i | 1 <= i < |boundaries|
-        ensures 0 < boundaries[i]
-      {
-        Integer_Order.IsStrictlySortedImpliesLt(boundaries, 0, i);
-      }
-    }
-  }
-
-  predicate ValidBoundariesForSeq(nkeys: int, boundaries: seq<nat>)
-    ensures ValidBoundariesForSeq(nkeys, boundaries) ==>
-    && (forall i :: 0 <= i < |boundaries|-1 ==> boundaries[i] < nkeys)
-    && (forall i :: 1 <= i < |boundaries| ==> 0 < boundaries[i])
-  {
-    ValidBoundariesForSeqBounds(nkeys, boundaries);
-    ValidBoundariesForSeqInner(nkeys, boundaries)
-  }
-  
-  lemma ValidBoundaryLength(nkeys: int, boundaries: seq<nat>)
-    requires ValidBoundariesForSeq(nkeys, boundaries)
-    ensures |boundaries| <= nkeys + 1
-  {
-    var i := 0;
-    while i < |boundaries|-1
-      invariant i <= |boundaries|-1
-      invariant i <= boundaries[i]
-    {
-      Integer_Order.IsStrictlySortedImpliesLt(boundaries, i, i+1);
-      i := i + 1;
-    }
-  }
-  
-  function {:opaque} ExtractBoundedSubsequence<T>(things: seq<T>, boundaries: seq<nat>, i: int) : seq<T>
-    requires ValidBoundariesForSeq(|things|, boundaries)
-    requires 0 <= i < |boundaries|-1
-  {
-    assert boundaries[i] <= boundaries[i+1] by
-    {
-      Integer_Order.IsStrictlySortedImpliesLte(boundaries, i, i+1);
-    }
-    things[boundaries[i]..boundaries[i+1]]
-  }
-
-  lemma ExtractBoundedSubsequenceLength<T>(things: seq<T>, boundaries: seq<nat>, i: int)
-    requires ValidBoundariesForSeq(|things|, boundaries)
-    requires 0 <= i < |boundaries|-1
-    ensures boundaries[i] <= boundaries[i+1];
-    ensures |ExtractBoundedSubsequence(things, boundaries, i)| == boundaries[i+1] - boundaries[i]
-  {
-    reveal_ExtractBoundedSubsequence();
-    Integer_Order.IsStrictlySortedImpliesLte(boundaries, i, i+1);
-  }
-  
-  // lemma ToSeqChildrenOfChildrenFromSeq(keys: seq<Key>, values: seq<Value>, boundaries: seq<nat>, children: seq<Node>)
-  //   requires |keys| == |values|
-  //   requires Keys.IsStrictlySorted(keys)
-  //   requires ValidBoundariesForSeq(|keys|, boundaries)
-  //   requires |boundaries| == |children| + 1
-  //   requires forall i :: 0 <= i < |children| ==> WF(children[i])
-  //   requires forall i :: 0 <= i < |children| ==> ToSeq(children[i]) == (ExtractBoundedSubsequence(keys, boundaries, i), ExtractBoundedSubsequence(values, boundaries, i))
-  //   ensures Flatten(ToSeqChildren(children).0) == keys
-  //   ensures Flatten(ToSeqChildren(children).1) == values
+  // predicate ValidBoundariesForSeqInner(nkeys: int, boundaries: seq<nat>)
   // {
-  //   if |children| == 1 {
-  //     ToSeqChildrenDecomposition(children);
-  //   } else {
-  //     var i := 0;
-  //     while i < |children|
-  //       invariant i <= |children|
-  //       invariant Flatten(ToSeqChildren(children[..i]).0) == keys[..boundaries[i]]
-  //       invariant Flatten(ToSeqChildren(children[..i]).1) == values[..boundaries[i]]
+  //   && 1 < |boundaries|
+  //   && boundaries[0] == 0
+  //   && Last(boundaries) == nkeys
+  //   && Integer_Order.IsStrictlySorted(boundaries)
+  // }
+
+  // lemma ValidBoundariesForSeqBounds(nkeys: int, boundaries: seq<nat>)
+  //   ensures ValidBoundariesForSeqInner(nkeys, boundaries) ==>
+  //   && (forall i :: 0 <= i < |boundaries|-1 ==> boundaries[i] < nkeys)
+  //   && (forall i :: 1 <= i < |boundaries| ==> 0 < boundaries[i])
+  // {
+  //   if ValidBoundariesForSeqInner(nkeys, boundaries) {
+  //     forall i | 0 <= i < |boundaries|-1
+  //       ensures boundaries[i] < nkeys
   //     {
-  //       ToSeqChildrenDecomposition(children[..i+1]);
-  //       assert children[..i] == children[..i+1][..i];
-  //       Integer_Order.IsStrictlySortedImpliesLte(boundaries, i, i+1);
-  //       assert keys[..boundaries[i+1]] == keys[..boundaries[i]] + ExtractBoundedSubsequence(keys, boundaries, i);
-  //       assert values[boundaries[i]..boundaries[i+1]] == ExtractBoundedSubsequence(values, boundaries, i);
-  //       assert values[..boundaries[i+1]] == values[..boundaries[i]] + ExtractBoundedSubsequence(values, boundaries, i);
-  //       i := i + 1;
+  //       Integer_Order.IsStrictlySortedImpliesLt(boundaries, i, |boundaries|-1);
   //     }
-  //     assert children[..|children|] == children;
-  //     assert keys[..boundaries[|children|]] == keys;
-  //     assert values[..boundaries[|children|]] == values;
+  //     forall i | 1 <= i < |boundaries|
+  //       ensures 0 < boundaries[i]
+  //     {
+  //       Integer_Order.IsStrictlySortedImpliesLt(boundaries, 0, i);
+  //     }
   //   }
   // }
 
-  // TODO: generalize KVLists and define equivalence in terms of their
-  // interpretation as maps.  (To handle key-message lists, we can
-  // break the merging process into a sorted-merge step and a
-  // message-amalgamation step.)  (robj)
-  // predicate TreeMatchesKVList(node: Node, kvlist: KVList)
-  //   requires WF(node)
-  //   requires WFKVList(kvlist)
+  // predicate ValidBoundariesForSeq(nkeys: int, boundaries: seq<nat>)
+  //   ensures ValidBoundariesForSeq(nkeys, boundaries) ==>
+  //   && (forall i :: 0 <= i < |boundaries|-1 ==> boundaries[i] < nkeys)
+  //   && (forall i :: 1 <= i < |boundaries| ==> 0 < boundaries[i])
   // {
-  //   Keys.SortedSeqForMap(Zip(kvlist.keys, kvlist.values), Interpretation(node))
+  //   ValidBoundariesForSeqBounds(nkeys, boundaries);
+  //   ValidBoundariesForSeqInner(nkeys, boundaries)
+  // }
+  
+  // lemma ValidBoundaryLength(nkeys: int, boundaries: seq<nat>)
+  //   requires ValidBoundariesForSeq(nkeys, boundaries)
+  //   ensures |boundaries| <= nkeys + 1
+  // {
+  //   var i := 0;
+  //   while i < |boundaries|-1
+  //     invariant i <= |boundaries|-1
+  //     invariant i <= boundaries[i]
+  //   {
+  //     Integer_Order.IsStrictlySortedImpliesLt(boundaries, i, i+1);
+  //     i := i + 1;
+  //   }
+  // }
+  
+  // function {:opaque} ExtractBoundedSubsequence<T>(things: seq<T>, boundaries: seq<nat>, i: int) : seq<T>
+  //   requires ValidBoundariesForSeq(|things|, boundaries)
+  //   requires 0 <= i < |boundaries|-1
+  // {
+  //   assert boundaries[i] <= boundaries[i+1] by
+  //   {
+  //     Integer_Order.IsStrictlySortedImpliesLte(boundaries, i, i+1);
+  //   }
+  //   things[boundaries[i]..boundaries[i+1]]
   // }
 
-  datatype Configuration = Configuration(ghost maxChildren: nat, ghost maxKeys: nat)
+  // lemma ExtractBoundedSubsequenceLength<T>(things: seq<T>, boundaries: seq<nat>, i: int)
+  //   requires ValidBoundariesForSeq(|things|, boundaries)
+  //   requires 0 <= i < |boundaries|-1
+  //   ensures boundaries[i] <= boundaries[i+1];
+  //   ensures |ExtractBoundedSubsequence(things, boundaries, i)| == boundaries[i+1] - boundaries[i]
+  // {
+  //   reveal_ExtractBoundedSubsequence();
+  //   Integer_Order.IsStrictlySortedImpliesLte(boundaries, i, i+1);
+  // }
+  
+  // // lemma ToSeqChildrenOfChildrenFromSeq(keys: seq<Key>, values: seq<Value>, boundaries: seq<nat>, children: seq<Node>)
+  // //   requires |keys| == |values|
+  // //   requires Keys.IsStrictlySorted(keys)
+  // //   requires ValidBoundariesForSeq(|keys|, boundaries)
+  // //   requires |boundaries| == |children| + 1
+  // //   requires forall i :: 0 <= i < |children| ==> WF(children[i])
+  // //   requires forall i :: 0 <= i < |children| ==> ToSeq(children[i]) == (ExtractBoundedSubsequence(keys, boundaries, i), ExtractBoundedSubsequence(values, boundaries, i))
+  // //   ensures Flatten(ToSeqChildren(children).0) == keys
+  // //   ensures Flatten(ToSeqChildren(children).1) == values
+  // // {
+  // //   if |children| == 1 {
+  // //     ToSeqChildrenDecomposition(children);
+  // //   } else {
+  // //     var i := 0;
+  // //     while i < |children|
+  // //       invariant i <= |children|
+  // //       invariant Flatten(ToSeqChildren(children[..i]).0) == keys[..boundaries[i]]
+  // //       invariant Flatten(ToSeqChildren(children[..i]).1) == values[..boundaries[i]]
+  // //     {
+  // //       ToSeqChildrenDecomposition(children[..i+1]);
+  // //       assert children[..i] == children[..i+1][..i];
+  // //       Integer_Order.IsStrictlySortedImpliesLte(boundaries, i, i+1);
+  // //       assert keys[..boundaries[i+1]] == keys[..boundaries[i]] + ExtractBoundedSubsequence(keys, boundaries, i);
+  // //       assert values[boundaries[i]..boundaries[i+1]] == ExtractBoundedSubsequence(values, boundaries, i);
+  // //       assert values[..boundaries[i+1]] == values[..boundaries[i]] + ExtractBoundedSubsequence(values, boundaries, i);
+  // //       i := i + 1;
+  // //     }
+  // //     assert children[..|children|] == children;
+  // //     assert keys[..boundaries[|children|]] == keys;
+  // //     assert values[..boundaries[|children|]] == values;
+  // //   }
+  // // }
 
-  predicate ValidConfiguration(config: Configuration)
-  {
-    && 0 < config.maxKeys
-    && 1 < config.maxChildren
-  }
+  // // TODO: generalize KVLists and define equivalence in terms of their
+  // // interpretation as maps.  (To handle key-message lists, we can
+  // // break the merging process into a sorted-merge step and a
+  // // message-amalgamation step.)  (robj)
+  // // predicate TreeMatchesKVList(node: Node, kvlist: KVList)
+  // //   requires WF(node)
+  // //   requires WFKVList(kvlist)
+  // // {
+  // //   Keys.SortedSeqForMap(Zip(kvlist.keys, kvlist.values), Interpretation(node))
+  // // }
+
+  // datatype Configuration = Configuration(ghost maxChildren: nat, ghost maxKeys: nat)
+
+  // predicate ValidConfiguration(config: Configuration)
+  // {
+  //   && 0 < config.maxKeys
+  //   && 1 < config.maxChildren
+  // }
     
-  predicate FitsConfig(node: Node, config: Configuration)
-  {
-    && WF(node)
-    && (if node.Index? then
-         && |node.children| <= config.maxChildren
-         && (forall i :: 0 <= i < |node.children| ==> FitsConfig(node.children[i], config))
-       else
-         && |node.keys| <= config.maxKeys
-      )
-  }
+  // predicate FitsConfig(node: Node, config: Configuration)
+  // {
+  //   && WF(node)
+  //   && (if node.Index? then
+  //        && |node.children| <= config.maxChildren
+  //        && (forall i :: 0 <= i < |node.children| ==> FitsConfig(node.children[i], config))
+  //      else
+  //        && |node.keys| <= config.maxKeys
+  //     )
+  // }
 
-  datatype KVList = KVList(keys: seq<Key>, values: seq<Value>)
+  // datatype KVList = KVList(keys: seq<Key>, values: seq<Value>)
   
-  predicate WFKVList(kvlist: KVList)
-  {
-    && |kvlist.keys| == |kvlist.values|
-    && Keys.IsStrictlySorted(kvlist.keys)
-  }
+  // predicate WFKVList(kvlist: KVList)
+  // {
+  //   && |kvlist.keys| == |kvlist.values|
+  //   && Keys.IsStrictlySorted(kvlist.keys)
+  // }
 
-  function KVListInterpretation(kvlist: KVList) : map<Key, Value>
-    requires WFKVList(kvlist)
-  {
-    var keys := Set(kvlist.keys);
-    map k | k in keys :: kvlist.values[Keys.LargestLte(kvlist.keys, k)]
-  }
+  // function KVListInterpretation(kvlist: KVList) : map<Key, Value>
+  //   requires WFKVList(kvlist)
+  // {
+  //   var keys := Set(kvlist.keys);
+  //   map k | k in keys :: kvlist.values[Keys.LargestLte(kvlist.keys, k)]
+  // }
   
-  function DropLastPiece<T>(things: seq<T>, boundaries: seq<nat>) : (subthings: seq<T>)
-    requires 2 < |boundaries|
-    requires ValidBoundariesForSeq(|things|, boundaries)
-    ensures ValidBoundariesForSeq(|subthings|, DropLast(boundaries))
-  {
-    Integer_Order.StrictlySortedSubsequence(boundaries, 0, |boundaries|-1);
-    things[..boundaries[|boundaries|-2]]
-  }
+  // function DropLastPiece<T>(things: seq<T>, boundaries: seq<nat>) : (subthings: seq<T>)
+  //   requires 2 < |boundaries|
+  //   requires ValidBoundariesForSeq(|things|, boundaries)
+  //   ensures ValidBoundariesForSeq(|subthings|, DropLast(boundaries))
+  // {
+  //   Integer_Order.StrictlySortedSubsequence(boundaries, 0, |boundaries|-1);
+  //   things[..boundaries[|boundaries|-2]]
+  // }
 
-  function DropLastKVListPiece(kvlist: KVList, boundaries: seq<nat>) : (sublist: KVList)
-    requires 2 < |boundaries|
-    requires WFKVList(kvlist)
-    requires ValidBoundariesForSeq(|kvlist.keys|, boundaries)
-    ensures ValidBoundariesForSeq(|sublist.keys|, DropLast(boundaries))
-    ensures WFKVList(sublist)
-  {
-    Keys.StrictlySortedSubsequence(kvlist.keys, 0, boundaries[|boundaries|-2]);
-    KVList(DropLastPiece(kvlist.keys, boundaries), DropLastPiece(kvlist.values, boundaries))
-  }
+  // function DropLastKVListPiece(kvlist: KVList, boundaries: seq<nat>) : (sublist: KVList)
+  //   requires 2 < |boundaries|
+  //   requires WFKVList(kvlist)
+  //   requires ValidBoundariesForSeq(|kvlist.keys|, boundaries)
+  //   ensures ValidBoundariesForSeq(|sublist.keys|, DropLast(boundaries))
+  //   ensures WFKVList(sublist)
+  // {
+  //   Keys.StrictlySortedSubsequence(kvlist.keys, 0, boundaries[|boundaries|-2]);
+  //   KVList(DropLastPiece(kvlist.keys, boundaries), DropLastPiece(kvlist.values, boundaries))
+  // }
 
-  function DropLastPivotsPiece(pivots: seq<Key>, boundaries: seq<nat>) : (subpivots: seq<Key>)
-    requires 2 < |boundaries|
-    requires ValidBoundariesForSeq(|pivots| + 1, boundaries)
-    ensures ValidBoundariesForSeq(|subpivots| + 1, DropLast(boundaries))
-  {
-    Integer_Order.StrictlySortedSubsequence(boundaries, 0, |boundaries|-1);
-    pivots[..boundaries[|boundaries|-2] - 1]
-  }
+  // function DropLastPivotsPiece(pivots: seq<Key>, boundaries: seq<nat>) : (subpivots: seq<Key>)
+  //   requires 2 < |boundaries|
+  //   requires ValidBoundariesForSeq(|pivots| + 1, boundaries)
+  //   ensures ValidBoundariesForSeq(|subpivots| + 1, DropLast(boundaries))
+  // {
+  //   Integer_Order.StrictlySortedSubsequence(boundaries, 0, |boundaries|-1);
+  //   pivots[..boundaries[|boundaries|-2] - 1]
+  // }
   
-  predicate {:opaque} BoundariesFit(boundaries: seq<nat>, groupSize: nat)
-  {
-    forall i :: 0 <= i < |boundaries| - 1 ==> boundaries[i+1] - boundaries[i] <= groupSize
-  }
+  // predicate {:opaque} BoundariesFit(boundaries: seq<nat>, groupSize: nat)
+  // {
+  //   forall i :: 0 <= i < |boundaries| - 1 ==> boundaries[i+1] - boundaries[i] <= groupSize
+  // }
   
-  function {:opaque} BuildBoundariesInner(numthings: nat, groupSize: nat) : (boundaries: seq<nat>)
-    requires 0 < numthings
-    requires 0 < groupSize
-  {
-    var tmp := Apply(i => i * groupSize, Range((numthings + groupSize - 1) / groupSize));
-    if Last(tmp) == numthings then tmp
-    else tmp + [numthings]
-  }
+  // function {:opaque} BuildBoundariesInner(numthings: nat, groupSize: nat) : (boundaries: seq<nat>)
+  //   requires 0 < numthings
+  //   requires 0 < groupSize
+  // {
+  //   var tmp := Apply(i => i * groupSize, Range((numthings + groupSize - 1) / groupSize));
+  //   if Last(tmp) == numthings then tmp
+  //   else tmp + [numthings]
+  // }
 
-  lemma BuildBoundariesProperties(numthings: nat, groupSize: nat)
-    requires 0 < numthings
-    requires 0 < groupSize
-    ensures ValidBoundariesForSeq(numthings, BuildBoundariesInner(numthings, groupSize))
-    ensures 1 < numthings && 1 < groupSize ==> |BuildBoundariesInner(numthings, groupSize)| - 1 < numthings
-    ensures BoundariesFit(BuildBoundariesInner(numthings, groupSize), groupSize)
-  {
-    reveal_BuildBoundariesInner();
-    reveal_BoundariesFit();
-    var tmp := Apply(i => i * groupSize, Range((numthings + groupSize - 1) / groupSize));
-    forall i, j | 0 <= i < j < |tmp|
-      ensures tmp[i] < tmp[j]
-    {
-      assert i * groupSize < j * groupSize;
-    }
-    Integer_Order.reveal_IsStrictlySorted();
-    if Last(tmp) == numthings {
-    } else {
-      Integer_Order.StrictlySortedAugment(tmp, numthings);
-      if 1 < numthings && 1 < groupSize {
-        Math.DivCeilLT(numthings, groupSize);
-      }
-    }
-  }
+  // lemma BuildBoundariesProperties(numthings: nat, groupSize: nat)
+  //   requires 0 < numthings
+  //   requires 0 < groupSize
+  //   ensures ValidBoundariesForSeq(numthings, BuildBoundariesInner(numthings, groupSize))
+  //   ensures 1 < numthings && 1 < groupSize ==> |BuildBoundariesInner(numthings, groupSize)| - 1 < numthings
+  //   ensures BoundariesFit(BuildBoundariesInner(numthings, groupSize), groupSize)
+  // {
+  //   reveal_BuildBoundariesInner();
+  //   reveal_BoundariesFit();
+  //   var tmp := Apply(i => i * groupSize, Range((numthings + groupSize - 1) / groupSize));
+  //   forall i, j | 0 <= i < j < |tmp|
+  //     ensures tmp[i] < tmp[j]
+  //   {
+  //     assert i * groupSize < j * groupSize;
+  //   }
+  //   Integer_Order.reveal_IsStrictlySorted();
+  //   if Last(tmp) == numthings {
+  //   } else {
+  //     Integer_Order.StrictlySortedAugment(tmp, numthings);
+  //     if 1 < numthings && 1 < groupSize {
+  //       Math.DivCeilLT(numthings, groupSize);
+  //     }
+  //   }
+  // }
 
-  function BuildBoundaries(numthings: nat, groupSize: nat) : (boundaries: seq<nat>)
-    requires 0 < numthings
-    requires 0 < groupSize
-    ensures ValidBoundariesForSeq(numthings, boundaries)
-    ensures 1 < numthings && 1 < groupSize ==> |BuildBoundaries(numthings, groupSize)| - 1 < numthings
-    ensures BoundariesFit(BuildBoundaries(numthings, groupSize), groupSize)
-  {
-    BuildBoundariesProperties(numthings, groupSize);
-    BuildBoundariesInner(numthings, groupSize)
-  }
+  // function BuildBoundaries(numthings: nat, groupSize: nat) : (boundaries: seq<nat>)
+  //   requires 0 < numthings
+  //   requires 0 < groupSize
+  //   ensures ValidBoundariesForSeq(numthings, boundaries)
+  //   ensures 1 < numthings && 1 < groupSize ==> |BuildBoundaries(numthings, groupSize)| - 1 < numthings
+  //   ensures BoundariesFit(BuildBoundaries(numthings, groupSize), groupSize)
+  // {
+  //   BuildBoundariesProperties(numthings, groupSize);
+  //   BuildBoundariesInner(numthings, groupSize)
+  // }
 
-  function {:opaque} ExtractPivotsForBoundaries(pivots: seq<Key>, boundaries: seq<nat>) : (subpivots: seq<Key>)
-    requires ValidBoundariesForSeq(|pivots|+1, boundaries)
-    ensures |subpivots| == |boundaries|-2
-  {
-    Apply(i
-          requires 0 <= i < |boundaries|-2
-          requires ValidBoundariesForSeq(|pivots|+1, boundaries) =>
-          Integer_Order.IsStrictlySortedImpliesLte(boundaries, i+1, |boundaries|-2);
-          pivots[boundaries[i+1]-1],
-          Range(|boundaries|-2))
-  }
+  // function {:opaque} ExtractPivotsForBoundaries(pivots: seq<Key>, boundaries: seq<nat>) : (subpivots: seq<Key>)
+  //   requires ValidBoundariesForSeq(|pivots|+1, boundaries)
+  //   ensures |subpivots| == |boundaries|-2
+  // {
+  //   Apply(i
+  //         requires 0 <= i < |boundaries|-2
+  //         requires ValidBoundariesForSeq(|pivots|+1, boundaries) =>
+  //         Integer_Order.IsStrictlySortedImpliesLte(boundaries, i+1, |boundaries|-2);
+  //         pivots[boundaries[i+1]-1],
+  //         Range(|boundaries|-2))
+  // }
 
-  lemma ExtractPivotsForBoundariesPreservesSort(pivots: seq<Key>, boundaries: seq<nat>)
-    requires ValidBoundariesForSeq(|pivots|+1, boundaries)
-    requires Keys.IsStrictlySorted(pivots)
-    ensures Keys.IsStrictlySorted(ExtractPivotsForBoundaries(pivots, boundaries))
-  {
-    reveal_ExtractPivotsForBoundaries();
-    var subpivots := ExtractPivotsForBoundaries(pivots, boundaries);
-    forall i, j | 0 <= i < j < |subpivots|
-      ensures Keys.lt(subpivots[i], subpivots[j])
-    {
-      var i' := boundaries[i+1]-1;
-      var j' := boundaries[j+1]-1;
-      Integer_Order.IsStrictlySortedImpliesLt(boundaries, i+1, j+1);
-      Keys.IsStrictlySortedImpliesLt(pivots, i', j');
-    }
-    Keys.reveal_IsStrictlySorted();
-  }
+  // lemma ExtractPivotsForBoundariesPreservesSort(pivots: seq<Key>, boundaries: seq<nat>)
+  //   requires ValidBoundariesForSeq(|pivots|+1, boundaries)
+  //   requires Keys.IsStrictlySorted(pivots)
+  //   ensures Keys.IsStrictlySorted(ExtractPivotsForBoundaries(pivots, boundaries))
+  // {
+  //   reveal_ExtractPivotsForBoundaries();
+  //   var subpivots := ExtractPivotsForBoundaries(pivots, boundaries);
+  //   forall i, j | 0 <= i < j < |subpivots|
+  //     ensures Keys.lt(subpivots[i], subpivots[j])
+  //   {
+  //     var i' := boundaries[i+1]-1;
+  //     var j' := boundaries[j+1]-1;
+  //     Integer_Order.IsStrictlySortedImpliesLt(boundaries, i+1, j+1);
+  //     Keys.IsStrictlySortedImpliesLt(pivots, i', j');
+  //   }
+  //   Keys.reveal_IsStrictlySorted();
+  // }
   
-  function ExtractPivotsFromKVList(kvlist: KVList) : (pivots: seq<Key>)
-    requires 0 < |kvlist.keys|
-    requires WFKVList(kvlist)
-    ensures Keys.IsStrictlySorted(pivots)
-  {
-    Keys.StrictlySortedSubsequence(kvlist.keys, 1, |kvlist.keys|);
-    assert kvlist.keys[1..] == kvlist.keys[1..|kvlist.keys|];
-    kvlist.keys[1..]
-  }
+  // function ExtractPivotsFromKVList(kvlist: KVList) : (pivots: seq<Key>)
+  //   requires 0 < |kvlist.keys|
+  //   requires WFKVList(kvlist)
+  //   ensures Keys.IsStrictlySorted(pivots)
+  // {
+  //   Keys.StrictlySortedSubsequence(kvlist.keys, 1, |kvlist.keys|);
+  //   assert kvlist.keys[1..] == kvlist.keys[1..|kvlist.keys|];
+  //   kvlist.keys[1..]
+  // }
 
-  function BuildLeafForSequence(kvlist: KVList, boundaries: seq<nat>, i: nat) : (node: Node)
-    requires WFKVList(kvlist)
-    requires ValidBoundariesForSeq(|kvlist.keys|, boundaries)
-    requires i < |boundaries|-1
-    ensures WF(node)
-    ensures AllKeys(node) != {}
-  {
-    var mykeys := ExtractBoundedSubsequence(kvlist.keys, boundaries, i);
-    var myvals := ExtractBoundedSubsequence(kvlist.values, boundaries, i);
-    Integer_Order.IsStrictlySortedImpliesLt(boundaries, i, i+1);
-    assert 0 < |mykeys| == |myvals| by { reveal_ExtractBoundedSubsequence(); }
-    assert Keys.IsStrictlySorted(mykeys) by {
-      reveal_ExtractBoundedSubsequence();
-      Keys.StrictlySortedSubsequence(kvlist.keys, boundaries[i], boundaries[i+1]);
-    }
-    var node := Leaf(mykeys, myvals);
-    Integer_Order.IsStrictlySortedImpliesLt(boundaries, i, i+1);
-    Keys.StrictlySortedSubsequence(kvlist.keys, boundaries[i], boundaries[i+1]);
-    //assert node.keys[0] in AllKeys(node) by { reveal_AllKeys(); }
-    assert 0 < |node.keys|;
-    node
-  }
+  // function BuildLeafForSequence(kvlist: KVList, boundaries: seq<nat>, i: nat) : (node: Node)
+  //   requires WFKVList(kvlist)
+  //   requires ValidBoundariesForSeq(|kvlist.keys|, boundaries)
+  //   requires i < |boundaries|-1
+  //   ensures WF(node)
+  //   ensures AllKeys(node) != {}
+  // {
+  //   var mykeys := ExtractBoundedSubsequence(kvlist.keys, boundaries, i);
+  //   var myvals := ExtractBoundedSubsequence(kvlist.values, boundaries, i);
+  //   Integer_Order.IsStrictlySortedImpliesLt(boundaries, i, i+1);
+  //   assert 0 < |mykeys| == |myvals| by { reveal_ExtractBoundedSubsequence(); }
+  //   assert Keys.IsStrictlySorted(mykeys) by {
+  //     reveal_ExtractBoundedSubsequence();
+  //     Keys.StrictlySortedSubsequence(kvlist.keys, boundaries[i], boundaries[i+1]);
+  //   }
+  //   var node := Leaf(mykeys, myvals);
+  //   Integer_Order.IsStrictlySortedImpliesLt(boundaries, i, i+1);
+  //   Keys.StrictlySortedSubsequence(kvlist.keys, boundaries[i], boundaries[i+1]);
+  //   //assert node.keys[0] in AllKeys(node) by { reveal_AllKeys(); }
+  //   assert 0 < |node.keys|;
+  //   node
+  // }
 
-  function BuildLeavesForSequenceInner(kvlist: KVList, boundaries: seq<nat>, count: nat) : (nodes: seq<Node>)
-    requires WFKVList(kvlist)
-    requires ValidBoundariesForSeq(|kvlist.keys|, boundaries)
-    requires count <= |boundaries|-1
-    ensures |nodes| == count
-    ensures forall i :: 0 <= i < |nodes| ==> nodes[i] == BuildLeafForSequence(kvlist, boundaries, i)
-    decreases count
-  {
-    if count == 0 then
-      []
-    else
-      BuildLeavesForSequenceInner(kvlist, boundaries, count-1) + [BuildLeafForSequence(kvlist, boundaries, count-1)]
-  }
+  // function BuildLeavesForSequenceInner(kvlist: KVList, boundaries: seq<nat>, count: nat) : (nodes: seq<Node>)
+  //   requires WFKVList(kvlist)
+  //   requires ValidBoundariesForSeq(|kvlist.keys|, boundaries)
+  //   requires count <= |boundaries|-1
+  //   ensures |nodes| == count
+  //   ensures forall i :: 0 <= i < |nodes| ==> nodes[i] == BuildLeafForSequence(kvlist, boundaries, i)
+  //   decreases count
+  // {
+  //   if count == 0 then
+  //     []
+  //   else
+  //     BuildLeavesForSequenceInner(kvlist, boundaries, count-1) + [BuildLeafForSequence(kvlist, boundaries, count-1)]
+  // }
   
-  function BuildLeavesForSequence(kvlist: KVList, boundaries: seq<nat>) : (nodes: seq<Node>)
-    requires WFKVList(kvlist)
-    requires ValidBoundariesForSeq(|kvlist.keys|, boundaries)
-    ensures |nodes| == |boundaries| - 1
-    ensures forall i :: 0 <= i < |nodes| ==> nodes[i] == BuildLeafForSequence(kvlist, boundaries, i)
-  {
-    BuildLeavesForSequenceInner(kvlist, boundaries, |boundaries|-1)
-  }
+  // function BuildLeavesForSequence(kvlist: KVList, boundaries: seq<nat>) : (nodes: seq<Node>)
+  //   requires WFKVList(kvlist)
+  //   requires ValidBoundariesForSeq(|kvlist.keys|, boundaries)
+  //   ensures |nodes| == |boundaries| - 1
+  //   ensures forall i :: 0 <= i < |nodes| ==> nodes[i] == BuildLeafForSequence(kvlist, boundaries, i)
+  // {
+  //   BuildLeavesForSequenceInner(kvlist, boundaries, |boundaries|-1)
+  // }
 
-  function BuildParent(children: seq<Node>, pivots: seq<Key>, boundaries: seq<nat>, i: nat) : (parent: Node)
-    requires WF(Index(pivots, children))
-    requires ValidBoundariesForSeq(|children|, boundaries)
-    requires 0 <= i < |boundaries|-1
-    ensures parent.Index?
-    ensures WF(parent)
-    ensures AllKeys(parent) != {}
-  {
-    ValidBoundariesForSeqBounds(|children|, boundaries);
-    Integer_Order.IsStrictlySortedImpliesLt(boundaries, i, i + 1);
-    var fparent := Index(pivots, children);
-    var parent := SubIndex(fparent, boundaries[i], boundaries[i+1]);
-    SubIndexPreservesWF(fparent, boundaries[i], boundaries[i+1]);
-    var wit :| wit in AllKeys(children[boundaries[i]]);
-    assert parent.children[0] == children[boundaries[i]];
-    assert wit in AllKeys(parent) by { reveal_AllKeys(); }
-    parent
-  }
+  // function BuildParent(children: seq<Node>, pivots: seq<Key>, boundaries: seq<nat>, i: nat) : (parent: Node)
+  //   requires WF(Index(pivots, children))
+  //   requires ValidBoundariesForSeq(|children|, boundaries)
+  //   requires 0 <= i < |boundaries|-1
+  //   ensures parent.Index?
+  //   ensures WF(parent)
+  //   ensures AllKeys(parent) != {}
+  // {
+  //   ValidBoundariesForSeqBounds(|children|, boundaries);
+  //   Integer_Order.IsStrictlySortedImpliesLt(boundaries, i, i + 1);
+  //   var fparent := Index(pivots, children);
+  //   var parent := SubIndex(fparent, boundaries[i], boundaries[i+1]);
+  //   SubIndexPreservesWF(fparent, boundaries[i], boundaries[i+1]);
+  //   var wit :| wit in AllKeys(children[boundaries[i]]);
+  //   assert parent.children[0] == children[boundaries[i]];
+  //   assert wit in AllKeys(parent) by { reveal_AllKeys(); }
+  //   parent
+  // }
 
-  lemma BuildParentAllKeys(children: seq<Node>, pivots: seq<Key>, boundaries: seq<nat>, i: nat)
-    requires WF(Index(pivots, children))
-    requires ValidBoundariesForSeq(|children|, boundaries)
-    requires 0 <= i < |boundaries|-1
-    ensures AllKeys(BuildParent(children, pivots, boundaries, i)) <= AllKeys(Index(pivots, children))
-  {
-    var parent := BuildParent(children, pivots, boundaries, i);
-    forall key | key in AllKeys(parent)
-      ensures key in AllKeys(Index(pivots, children))
-    {
-      reveal_AllKeys();
-      if j :| 0 <= j < |parent.pivots| && key == parent.pivots[j] {
-      } else {
-        Integer_Order.IsStrictlySortedImpliesLt(boundaries, i, i+1);
-      }
-    }
-  }
+  // lemma BuildParentAllKeys(children: seq<Node>, pivots: seq<Key>, boundaries: seq<nat>, i: nat)
+  //   requires WF(Index(pivots, children))
+  //   requires ValidBoundariesForSeq(|children|, boundaries)
+  //   requires 0 <= i < |boundaries|-1
+  //   ensures AllKeys(BuildParent(children, pivots, boundaries, i)) <= AllKeys(Index(pivots, children))
+  // {
+  //   var parent := BuildParent(children, pivots, boundaries, i);
+  //   forall key | key in AllKeys(parent)
+  //     ensures key in AllKeys(Index(pivots, children))
+  //   {
+  //     reveal_AllKeys();
+  //     if j :| 0 <= j < |parent.pivots| && key == parent.pivots[j] {
+  //     } else {
+  //       Integer_Order.IsStrictlySortedImpliesLt(boundaries, i, i+1);
+  //     }
+  //   }
+  // }
   
   
-  function BuildParentsInner(children: seq<Node>, pivots: seq<Key>, boundaries: seq<nat>, count: nat) :
-    (parents: seq<Node>)
-    requires WF(Index(pivots, children))
-    requires ValidBoundariesForSeq(|children|, boundaries)
-    requires 0 <= count <= |boundaries|-1
-    ensures |parents| == count
-    ensures forall i :: 0 <= i < |parents| ==> parents[i].Index?
-    ensures forall i :: 0 <= i < |parents| ==> WF(parents[i])
-    ensures forall i :: 0 <= i < |parents| ==> AllKeys(parents[i]) != {}
-  {
-    if count == 0 then
-      []
-    else
-      BuildParentsInner(children, pivots, boundaries, count-1) +
-      [BuildParent(children, pivots, boundaries, count-1)]
-  }
+  // function BuildParentsInner(children: seq<Node>, pivots: seq<Key>, boundaries: seq<nat>, count: nat) :
+  //   (parents: seq<Node>)
+  //   requires WF(Index(pivots, children))
+  //   requires ValidBoundariesForSeq(|children|, boundaries)
+  //   requires 0 <= count <= |boundaries|-1
+  //   ensures |parents| == count
+  //   ensures forall i :: 0 <= i < |parents| ==> parents[i].Index?
+  //   ensures forall i :: 0 <= i < |parents| ==> WF(parents[i])
+  //   ensures forall i :: 0 <= i < |parents| ==> AllKeys(parents[i]) != {}
+  // {
+  //   if count == 0 then
+  //     []
+  //   else
+  //     BuildParentsInner(children, pivots, boundaries, count-1) +
+  //     [BuildParent(children, pivots, boundaries, count-1)]
+  // }
 
-  lemma BuildParentsInnerProperties(children: seq<Node>, pivots: seq<Key>, boundaries: seq<nat>, count: nat, parents: seq<Node>)
-    requires WF(Index(pivots, children))
-    requires ValidBoundariesForSeq(|children|, boundaries)
-    requires 0 <= count <= |boundaries|-1
-    requires parents == BuildParentsInner(children, pivots, boundaries, count)
-    ensures forall i :: 0 <= i < |parents| ==> boundaries[i] < boundaries[i+1]
-    ensures forall i :: 0 <= i < |parents| ==> parents[i].pivots == pivots[boundaries[i]..boundaries[i+1]-1];
-    ensures forall i :: 0 <= i < |parents| ==> parents[i].children == children[boundaries[i]..boundaries[i+1]];
-  {
-    forall i | 0 <= i < |parents|
-      ensures boundaries[i] < boundaries[i+1]
-    {
-      Integer_Order.IsStrictlySortedImpliesLt(boundaries, i, i+1);
-    }
+  // lemma BuildParentsInnerProperties(children: seq<Node>, pivots: seq<Key>, boundaries: seq<nat>, count: nat, parents: seq<Node>)
+  //   requires WF(Index(pivots, children))
+  //   requires ValidBoundariesForSeq(|children|, boundaries)
+  //   requires 0 <= count <= |boundaries|-1
+  //   requires parents == BuildParentsInner(children, pivots, boundaries, count)
+  //   ensures forall i :: 0 <= i < |parents| ==> boundaries[i] < boundaries[i+1]
+  //   ensures forall i :: 0 <= i < |parents| ==> parents[i].pivots == pivots[boundaries[i]..boundaries[i+1]-1];
+  //   ensures forall i :: 0 <= i < |parents| ==> parents[i].children == children[boundaries[i]..boundaries[i+1]];
+  // {
+  //   forall i | 0 <= i < |parents|
+  //     ensures boundaries[i] < boundaries[i+1]
+  //   {
+  //     Integer_Order.IsStrictlySortedImpliesLt(boundaries, i, i+1);
+  //   }
 
-    if count == 0 {
-    } else {
-      BuildParentsInnerProperties(children, pivots, boundaries, count-1, DropLast(parents));
-    }
-  }
+  //   if count == 0 {
+  //   } else {
+  //     BuildParentsInnerProperties(children, pivots, boundaries, count-1, DropLast(parents));
+  //   }
+  // }
 
-  function BuildParents(children: seq<Node>, pivots: seq<Key>, boundaries: seq<nat>) :
-    (parents: seq<Node>)
-    requires WF(Index(pivots, children))
-    requires ValidBoundariesForSeq(|children|, boundaries)
-    ensures forall i :: 0 <= i < |parents| ==> parents[i].Index?
-    ensures forall i :: 0 <= i < |parents| ==> WF(parents[i])
-    ensures forall i :: 0 <= i < |parents| ==> AllKeys(parents[i]) != {}
-  {
-    BuildParentsInner(children, pivots, boundaries, |boundaries| - 1)
-  }
+  // function BuildParents(children: seq<Node>, pivots: seq<Key>, boundaries: seq<nat>) :
+  //   (parents: seq<Node>)
+  //   requires WF(Index(pivots, children))
+  //   requires ValidBoundariesForSeq(|children|, boundaries)
+  //   ensures forall i :: 0 <= i < |parents| ==> parents[i].Index?
+  //   ensures forall i :: 0 <= i < |parents| ==> WF(parents[i])
+  //   ensures forall i :: 0 <= i < |parents| ==> AllKeys(parents[i]) != {}
+  // {
+  //   BuildParentsInner(children, pivots, boundaries, |boundaries| - 1)
+  // }
 
-  function Grandparent(children: seq<Node>, pivots: seq<Key>, boundaries: seq<nat>) : (grandparent: Node)
-    requires WF(Index(pivots, children))
-    requires ValidBoundariesForSeq(|children|, boundaries)
-  {
-    Index(ExtractPivotsForBoundaries(pivots, boundaries), BuildParents(children, pivots, boundaries))
-  }
+  // function Grandparent(children: seq<Node>, pivots: seq<Key>, boundaries: seq<nat>) : (grandparent: Node)
+  //   requires WF(Index(pivots, children))
+  //   requires ValidBoundariesForSeq(|children|, boundaries)
+  // {
+  //   Index(ExtractPivotsForBoundaries(pivots, boundaries), BuildParents(children, pivots, boundaries))
+  // }
   
-  lemma GrandparentWF(children: seq<Node>, pivots: seq<Key>, boundaries: seq<nat>)
-    requires WF(Index(pivots, children))
-    requires ValidBoundariesForSeq(|children|, boundaries)
-    ensures WF(Grandparent(children, pivots, boundaries))
-    //ensures Interpretation(Grandparent(children, pivots, boundaries)) == Interpretation(Index(pivots, children))
-  {
-    var oldparent := Index(pivots, children);
-    var grandparent := Grandparent(children, pivots, boundaries);
-    BuildParentsInnerProperties(children, pivots, boundaries, |boundaries|-1, grandparent.children);
+  // lemma GrandparentWF(children: seq<Node>, pivots: seq<Key>, boundaries: seq<nat>)
+  //   requires WF(Index(pivots, children))
+  //   requires ValidBoundariesForSeq(|children|, boundaries)
+  //   ensures WF(Grandparent(children, pivots, boundaries))
+  //   //ensures Interpretation(Grandparent(children, pivots, boundaries)) == Interpretation(Index(pivots, children))
+  // {
+  //   var oldparent := Index(pivots, children);
+  //   var grandparent := Grandparent(children, pivots, boundaries);
+  //   BuildParentsInnerProperties(children, pivots, boundaries, |boundaries|-1, grandparent.children);
     
-    ExtractPivotsForBoundariesPreservesSort(pivots, boundaries);
-    forall i | 0 <= i < |grandparent.children|-1
-      ensures AllKeysBelowBound(grandparent, i)
-    {
-      forall key | key in AllKeys(grandparent.children[i])
-        ensures Keys.lt(key, grandparent.pivots[i])
-      {
-        assert grandparent.pivots[i] == pivots[boundaries[i+1]-1] by { reveal_ExtractPivotsForBoundaries(); }
-        var parent := grandparent.children[i];
-        reveal_AllKeys();
-        if j :| 0 <= j < |parent.pivots| && key == parent.pivots[j] {
-          Keys.IsStrictlySortedImpliesLt(pivots, boundaries[i] + j, boundaries[i+1]-1);
-        } else {
-          var j :| 0 <= j < |parent.children| && key in AllKeys(parent.children[j]);
-          assert AllKeysBelowBound(oldparent, boundaries[i] + j);
-          Keys.IsStrictlySortedImpliesLte(pivots, boundaries[i] + j, boundaries[i+1]-1);
-        }
-      }
-    }
-    forall i | 0 < i < |grandparent.children|
-      ensures AllKeysAboveBound(grandparent, i)
-    {
-      forall key | key in AllKeys(grandparent.children[i])
-        ensures Keys.lte(grandparent.pivots[i-1], key)
-      {
-        assert grandparent.pivots[i-1] == pivots[boundaries[i]-1] by { reveal_ExtractPivotsForBoundaries(); }
-        var parent := grandparent.children[i];
-        reveal_AllKeys();
-        if j :| 0 <= j < |parent.pivots| && key == parent.pivots[j] {
-          assert boundaries[i] + j < boundaries[i+1];
-          Keys.IsStrictlySortedImpliesLt(pivots, boundaries[i]-1, boundaries[i] + j);
-        } else {
-          var j :| 0 <= j < |parent.children| && key in AllKeys(parent.children[j]);
-          assert boundaries[i] + j < boundaries[i+1];
-          assert AllKeysAboveBound(oldparent, boundaries[i] + j);
-          Keys.IsStrictlySortedImpliesLte(pivots, boundaries[i]-1, boundaries[i] + j-1);
-        }
-      }
-    }
-    assert WF(grandparent);
-  }
+  //   ExtractPivotsForBoundariesPreservesSort(pivots, boundaries);
+  //   forall i | 0 <= i < |grandparent.children|-1
+  //     ensures AllKeysBelowBound(grandparent, i)
+  //   {
+  //     forall key | key in AllKeys(grandparent.children[i])
+  //       ensures Keys.lt(key, grandparent.pivots[i])
+  //     {
+  //       assert grandparent.pivots[i] == pivots[boundaries[i+1]-1] by { reveal_ExtractPivotsForBoundaries(); }
+  //       var parent := grandparent.children[i];
+  //       reveal_AllKeys();
+  //       if j :| 0 <= j < |parent.pivots| && key == parent.pivots[j] {
+  //         Keys.IsStrictlySortedImpliesLt(pivots, boundaries[i] + j, boundaries[i+1]-1);
+  //       } else {
+  //         var j :| 0 <= j < |parent.children| && key in AllKeys(parent.children[j]);
+  //         assert AllKeysBelowBound(oldparent, boundaries[i] + j);
+  //         Keys.IsStrictlySortedImpliesLte(pivots, boundaries[i] + j, boundaries[i+1]-1);
+  //       }
+  //     }
+  //   }
+  //   forall i | 0 < i < |grandparent.children|
+  //     ensures AllKeysAboveBound(grandparent, i)
+  //   {
+  //     forall key | key in AllKeys(grandparent.children[i])
+  //       ensures Keys.lte(grandparent.pivots[i-1], key)
+  //     {
+  //       assert grandparent.pivots[i-1] == pivots[boundaries[i]-1] by { reveal_ExtractPivotsForBoundaries(); }
+  //       var parent := grandparent.children[i];
+  //       reveal_AllKeys();
+  //       if j :| 0 <= j < |parent.pivots| && key == parent.pivots[j] {
+  //         assert boundaries[i] + j < boundaries[i+1];
+  //         Keys.IsStrictlySortedImpliesLt(pivots, boundaries[i]-1, boundaries[i] + j);
+  //       } else {
+  //         var j :| 0 <= j < |parent.children| && key in AllKeys(parent.children[j]);
+  //         assert boundaries[i] + j < boundaries[i+1];
+  //         assert AllKeysAboveBound(oldparent, boundaries[i] + j);
+  //         Keys.IsStrictlySortedImpliesLte(pivots, boundaries[i]-1, boundaries[i] + j-1);
+  //       }
+  //     }
+  //   }
+  //   assert WF(grandparent);
+  // }
 
-  lemma GrandparentAllKeys(children: seq<Node>, pivots: seq<Key>, boundaries: seq<nat>)
-    requires WF(Index(pivots, children))
-    requires ValidBoundariesForSeq(|children|, boundaries)
-    ensures AllKeys(Grandparent(children, pivots, boundaries)) == AllKeys(Index(pivots, children))
-  {
-    var oldparent := Index(pivots, children);
-    var grandparent := Grandparent(children, pivots, boundaries);
-    BuildParentsInnerProperties(children, pivots, boundaries, |boundaries|-1, grandparent.children);
+  // lemma GrandparentAllKeys(children: seq<Node>, pivots: seq<Key>, boundaries: seq<nat>)
+  //   requires WF(Index(pivots, children))
+  //   requires ValidBoundariesForSeq(|children|, boundaries)
+  //   ensures AllKeys(Grandparent(children, pivots, boundaries)) == AllKeys(Index(pivots, children))
+  // {
+  //   var oldparent := Index(pivots, children);
+  //   var grandparent := Grandparent(children, pivots, boundaries);
+  //   BuildParentsInnerProperties(children, pivots, boundaries, |boundaries|-1, grandparent.children);
 
-    var grandak := AllKeys(grandparent);
-    var oldak := AllKeys(oldparent);
+  //   var grandak := AllKeys(grandparent);
+  //   var oldak := AllKeys(oldparent);
     
-    forall key | key in grandak
-      ensures key in oldak
-    {
-      reveal_AllKeys();
-      if j :| 0 <= j < |grandparent.pivots| && key == grandparent.pivots[j] {
-        assert key == pivots[boundaries[j+1] - 1] by { reveal_ExtractPivotsForBoundaries(); }
-      } else {
-        var j :| 0 <= j < |grandparent.children| && key in AllKeys(grandparent.children[j]);
-        BuildParentAllKeys(children, pivots, boundaries, j);
-      }
-    }
+  //   forall key | key in grandak
+  //     ensures key in oldak
+  //   {
+  //     reveal_AllKeys();
+  //     if j :| 0 <= j < |grandparent.pivots| && key == grandparent.pivots[j] {
+  //       assert key == pivots[boundaries[j+1] - 1] by { reveal_ExtractPivotsForBoundaries(); }
+  //     } else {
+  //       var j :| 0 <= j < |grandparent.children| && key in AllKeys(grandparent.children[j]);
+  //       BuildParentAllKeys(children, pivots, boundaries, j);
+  //     }
+  //   }
 
-    forall key | key in oldak
-      ensures key in grandak
-    {
-      reveal_AllKeys();
-      if j :| 0 <= j < |pivots| && key == pivots[j] {
-        var i := Integer_Order.LargestLte(boundaries, j);
-        if j == boundaries[i+1]-1 {
-          assert key == grandparent.pivots[i] by { reveal_ExtractPivotsForBoundaries(); }
-        } else {
-          assert grandparent.children[i].pivots == pivots[boundaries[i]..boundaries[i+1]-1];
-          assert key == grandparent.children[i].pivots[j - boundaries[i]];
-          assert key in AllKeys(grandparent.children[i]);
-        }
-      } else {
-        var j :| 0 <= j < |children| && key in AllKeys(children[j]);
-        var i := Integer_Order.LargestLte(boundaries, j);
-        assert grandparent.children[i].children == children[boundaries[i]..boundaries[i+1]];
-        assert key in AllKeys(grandparent.children[i]);
-      }
+  //   forall key | key in oldak
+  //     ensures key in grandak
+  //   {
+  //     reveal_AllKeys();
+  //     if j :| 0 <= j < |pivots| && key == pivots[j] {
+  //       var i := Integer_Order.LargestLte(boundaries, j);
+  //       if j == boundaries[i+1]-1 {
+  //         assert key == grandparent.pivots[i] by { reveal_ExtractPivotsForBoundaries(); }
+  //       } else {
+  //         assert grandparent.children[i].pivots == pivots[boundaries[i]..boundaries[i+1]-1];
+  //         assert key == grandparent.children[i].pivots[j - boundaries[i]];
+  //         assert key in AllKeys(grandparent.children[i]);
+  //       }
+  //     } else {
+  //       var j :| 0 <= j < |children| && key in AllKeys(children[j]);
+  //       var i := Integer_Order.LargestLte(boundaries, j);
+  //       assert grandparent.children[i].children == children[boundaries[i]..boundaries[i+1]];
+  //       assert key in AllKeys(grandparent.children[i]);
+  //     }
       
-    }
-  }
+  //   }
+  // }
   
-  lemma GrandparentInterpretation(children: seq<Node>, pivots: seq<Key>, boundaries: seq<nat>)
-    requires WF(Index(pivots, children))
-    requires ValidBoundariesForSeq(|children|, boundaries)
-    ensures WF(Grandparent(children, pivots, boundaries))
-    ensures Interpretation(Grandparent(children, pivots, boundaries)) == Interpretation(Index(pivots, children))
-  {
-    var oldparent := Index(pivots, children);
-    var grandparent := Grandparent(children, pivots, boundaries);
-    BuildParentsInnerProperties(children, pivots, boundaries, |boundaries|-1, grandparent.children);
-    GrandparentWF(children, pivots, boundaries);
+  // lemma GrandparentInterpretation(children: seq<Node>, pivots: seq<Key>, boundaries: seq<nat>)
+  //   requires WF(Index(pivots, children))
+  //   requires ValidBoundariesForSeq(|children|, boundaries)
+  //   ensures WF(Grandparent(children, pivots, boundaries))
+  //   ensures Interpretation(Grandparent(children, pivots, boundaries)) == Interpretation(Index(pivots, children))
+  // {
+  //   var oldparent := Index(pivots, children);
+  //   var grandparent := Grandparent(children, pivots, boundaries);
+  //   BuildParentsInnerProperties(children, pivots, boundaries, |boundaries|-1, grandparent.children);
+  //   GrandparentWF(children, pivots, boundaries);
     
-    var grandinterp := Interpretation(grandparent);
-    var oldinterp := Interpretation(oldparent);
+  //   var grandinterp := Interpretation(grandparent);
+  //   var oldinterp := Interpretation(oldparent);
 
-    forall key | key in grandinterp
-      ensures MapsTo(oldinterp, key, grandinterp[key])
-    {
-      var i := Keys.LargestLte(grandparent.pivots, key) + 1;
-      InterpretationInheritance(grandparent, key);
-      var j := Keys.LargestLte(grandparent.children[i].pivots, key) + 1;
-      InterpretationInheritance(grandparent.children[i], key);
-      assert boundaries[i] + j < boundaries[i+1];
-      assert key in Interpretation(children[boundaries[i] + j]);
-      AllKeysIsConsistentWithInterpretation(children[boundaries[i] + j], key);
-      if 0 < boundaries[i] + j {
-        assert AllKeysAboveBound(oldparent, boundaries[i] + j);
-      }
-      if boundaries[i] + j < |children|-1 {
-        assert AllKeysBelowBound(oldparent, boundaries[i] + j);
-      }
-      Keys.LargestLteIsUnique2(pivots, key, boundaries[i] + j - 1);
-      InterpretationDelegation(oldparent, key);
-    }
+  //   forall key | key in grandinterp
+  //     ensures MapsTo(oldinterp, key, grandinterp[key])
+  //   {
+  //     var i := Keys.LargestLte(grandparent.pivots, key) + 1;
+  //     InterpretationInheritance(grandparent, key);
+  //     var j := Keys.LargestLte(grandparent.children[i].pivots, key) + 1;
+  //     InterpretationInheritance(grandparent.children[i], key);
+  //     assert boundaries[i] + j < boundaries[i+1];
+  //     assert key in Interpretation(children[boundaries[i] + j]);
+  //     AllKeysIsConsistentWithInterpretation(children[boundaries[i] + j], key);
+  //     if 0 < boundaries[i] + j {
+  //       assert AllKeysAboveBound(oldparent, boundaries[i] + j);
+  //     }
+  //     if boundaries[i] + j < |children|-1 {
+  //       assert AllKeysBelowBound(oldparent, boundaries[i] + j);
+  //     }
+  //     Keys.LargestLteIsUnique2(pivots, key, boundaries[i] + j - 1);
+  //     InterpretationDelegation(oldparent, key);
+  //   }
     
-    forall key | key in oldinterp
-      ensures key in grandinterp
-    {
-      var j := Keys.LargestLte(pivots, key) + 1;
-      InterpretationInheritance(oldparent, key);
-      var i := Integer_Order.LargestLte(boundaries, j);
-      var j' := j - boundaries[i];
-      AllKeysIsConsistentWithInterpretation(children[j], key);
-      assert grandparent.children[i].children == children[boundaries[i]..boundaries[i+1]];
-      assert grandparent.children[i].pivots == pivots[boundaries[i]..boundaries[i+1]-1];
-      if 0 < j {
-        assert AllKeysAboveBound(oldparent, j);
-        assert Keys.lte(pivots[j-1], key);
-      }
-      if j' < |grandparent.children[i].pivots| {
-        assert AllKeysBelowBound(oldparent, j);
-        assert grandparent.children[i].pivots[j'] == pivots[j];
-        assert Keys.lt(key, grandparent.children[i].pivots[j']);
-      }
-      Keys.LargestLteIsUnique2(grandparent.children[i].pivots, key, j' as int - 1);
-      InterpretationDelegation(grandparent.children[i], key);
+  //   forall key | key in oldinterp
+  //     ensures key in grandinterp
+  //   {
+  //     var j := Keys.LargestLte(pivots, key) + 1;
+  //     InterpretationInheritance(oldparent, key);
+  //     var i := Integer_Order.LargestLte(boundaries, j);
+  //     var j' := j - boundaries[i];
+  //     AllKeysIsConsistentWithInterpretation(children[j], key);
+  //     assert grandparent.children[i].children == children[boundaries[i]..boundaries[i+1]];
+  //     assert grandparent.children[i].pivots == pivots[boundaries[i]..boundaries[i+1]-1];
+  //     if 0 < j {
+  //       assert AllKeysAboveBound(oldparent, j);
+  //       assert Keys.lte(pivots[j-1], key);
+  //     }
+  //     if j' < |grandparent.children[i].pivots| {
+  //       assert AllKeysBelowBound(oldparent, j);
+  //       assert grandparent.children[i].pivots[j'] == pivots[j];
+  //       assert Keys.lt(key, grandparent.children[i].pivots[j']);
+  //     }
+  //     Keys.LargestLteIsUnique2(grandparent.children[i].pivots, key, j' as int - 1);
+  //     InterpretationDelegation(grandparent.children[i], key);
 
-      AllKeysIsConsistentWithInterpretation(grandparent.children[i], key);
-      if 0 < i {
-        assert AllKeysAboveBound(grandparent, i);
-      }
-      if i < |grandparent.children|-1 {
-        assert AllKeysBelowBound(grandparent, i);
-      }
-      Keys.LargestLteIsUnique2(grandparent.pivots, key, i - 1);
-      InterpretationDelegation(grandparent, key);
-    }
-  }
+  //     AllKeysIsConsistentWithInterpretation(grandparent.children[i], key);
+  //     if 0 < i {
+  //       assert AllKeysAboveBound(grandparent, i);
+  //     }
+  //     if i < |grandparent.children|-1 {
+  //       assert AllKeysBelowBound(grandparent, i);
+  //     }
+  //     Keys.LargestLteIsUnique2(grandparent.pivots, key, i - 1);
+  //     InterpretationDelegation(grandparent, key);
+  //   }
+  // }
 
-  lemma ParentsFitConfig(children: seq<Node>, pivots: seq<Key>, boundaries: seq<nat>, config: Configuration)
-    requires WF(Index(pivots, children))
-    requires ValidBoundariesForSeq(|children|, boundaries)
-    requires ValidConfiguration(config)
-    requires forall i :: 0 <= i < |children| ==> FitsConfig(children[i], config)
-    requires BoundariesFit(boundaries, config.maxChildren)
-    ensures forall i :: 0 <= i < |BuildParents(children, pivots, boundaries)| ==>
-      FitsConfig(BuildParents(children, pivots, boundaries)[i], config)
-  {
-    var parents := BuildParents(children, pivots, boundaries);
-    BuildParentsInnerProperties(children, pivots, boundaries, |boundaries|-1, parents);
-    reveal_BoundariesFit();
-    forall i | 0 <= i < |parents|
-      ensures FitsConfig(parents[i], config)
-    {
-      assert |parents[i].children| == boundaries[i+1] - boundaries[i];
-    }
-  }
+  // lemma ParentsFitConfig(children: seq<Node>, pivots: seq<Key>, boundaries: seq<nat>, config: Configuration)
+  //   requires WF(Index(pivots, children))
+  //   requires ValidBoundariesForSeq(|children|, boundaries)
+  //   requires ValidConfiguration(config)
+  //   requires forall i :: 0 <= i < |children| ==> FitsConfig(children[i], config)
+  //   requires BoundariesFit(boundaries, config.maxChildren)
+  //   ensures forall i :: 0 <= i < |BuildParents(children, pivots, boundaries)| ==>
+  //     FitsConfig(BuildParents(children, pivots, boundaries)[i], config)
+  // {
+  //   var parents := BuildParents(children, pivots, boundaries);
+  //   BuildParentsInnerProperties(children, pivots, boundaries, |boundaries|-1, parents);
+  //   reveal_BoundariesFit();
+  //   forall i | 0 <= i < |parents|
+  //     ensures FitsConfig(parents[i], config)
+  //   {
+  //     assert |parents[i].children| == boundaries[i+1] - boundaries[i];
+  //   }
+  // }
 
-  // This function clumps node.children together into config-sized parents,
-  // recursing until there's only one node left.
-  function BuildLayers(children: seq<Node>, pivots: seq<Key>, config: Configuration) : (newnode: Node)
-    requires WF(Index(pivots, children))
-    requires ValidConfiguration(config)
-    requires forall i :: 0 <= i < |children| ==> FitsConfig(children[i], config)
-    ensures WF(newnode)
-    ensures AllKeys(newnode) == AllKeys(Index(pivots, children))
-    ensures Interpretation(newnode) == Interpretation(Index(pivots, children))
-    ensures FitsConfig(newnode, config)
-    decreases |children|
-  {
-    reveal_Interpretation();
-    if |children| == 1  then
-      GrowPreservesAllKeys(children[0]);
-      assert children == [children[0]];
-      GrowPreservesInterpretation(children[0]);
-      children[0]
-    else
-      var boundaries := BuildBoundaries(|children|, config.maxChildren);
-      var parents := BuildParents(children, pivots, boundaries);
-      var ppivots := ExtractPivotsForBoundaries(pivots, boundaries);
-      GrandparentWF(children, pivots, boundaries);
-      GrandparentAllKeys(children, pivots, boundaries);
-      GrandparentInterpretation(children, pivots, boundaries);
-      ParentsFitConfig(children, pivots, boundaries, config);
-      BuildLayers(parents, ppivots, config)
-  }
+  // // This function clumps node.children together into config-sized parents,
+  // // recursing until there's only one node left.
+  // function BuildLayers(children: seq<Node>, pivots: seq<Key>, config: Configuration) : (newnode: Node)
+  //   requires WF(Index(pivots, children))
+  //   requires ValidConfiguration(config)
+  //   requires forall i :: 0 <= i < |children| ==> FitsConfig(children[i], config)
+  //   ensures WF(newnode)
+  //   ensures AllKeys(newnode) == AllKeys(Index(pivots, children))
+  //   ensures Interpretation(newnode) == Interpretation(Index(pivots, children))
+  //   ensures FitsConfig(newnode, config)
+  //   decreases |children|
+  // {
+  //   reveal_Interpretation();
+  //   if |children| == 1  then
+  //     GrowPreservesAllKeys(children[0]);
+  //     assert children == [children[0]];
+  //     GrowPreservesInterpretation(children[0]);
+  //     children[0]
+  //   else
+  //     var boundaries := BuildBoundaries(|children|, config.maxChildren);
+  //     var parents := BuildParents(children, pivots, boundaries);
+  //     var ppivots := ExtractPivotsForBoundaries(pivots, boundaries);
+  //     GrandparentWF(children, pivots, boundaries);
+  //     GrandparentAllKeys(children, pivots, boundaries);
+  //     GrandparentInterpretation(children, pivots, boundaries);
+  //     ParentsFitConfig(children, pivots, boundaries, config);
+  //     BuildLayers(parents, ppivots, config)
+  // }
 
-  lemma LeavesProperties(kvlist: KVList, config: Configuration, boundaries: seq<nat>, node: Node)
-    requires 0 < |kvlist.keys|
-    requires WFKVList(kvlist)
-    requires ValidConfiguration(config)
-    requires boundaries == BuildBoundaries(|kvlist.keys|, config.maxKeys)
-    requires node.Index?
-    requires node.children == BuildLeavesForSequence(kvlist, boundaries)
-    requires node.pivots == ExtractPivotsForBoundaries(ExtractPivotsFromKVList(kvlist), boundaries)
-    ensures WF(node)
-    ensures Interpretation(node) == KVListInterpretation(kvlist)
-    ensures forall i :: 0 <= i < |node.children| ==> FitsConfig(node.children[i], config)
-  {
-    ExtractPivotsForBoundariesPreservesSort(ExtractPivotsFromKVList(kvlist), boundaries);
-    reveal_ExtractPivotsForBoundaries();
-    forall i | 0 <= i < |node.children| - 1
-      ensures AllKeysBelowBound(node, i)
-    {
-      forall j | 0 <= j < |node.children[i].keys|
-        ensures Keys.lt(node.children[i].keys[j], node.pivots[i])
-      {
-        reveal_ExtractBoundedSubsequence();
-        ExtractBoundedSubsequenceLength(kvlist.keys, boundaries, i);
-        Keys.IsStrictlySortedImpliesLt(kvlist.keys, boundaries[i] + j, boundaries[i+1]);
-      }
-      reveal_AllKeys();
-    }
-    forall i | 0 < i < |node.children|
-      ensures AllKeysAboveBound(node, i)
-    {
-      forall j | 0 <= j < |node.children[i].keys|
-        ensures Keys.lte(node.pivots[i-1], node.children[i].keys[j])
-      {
-        reveal_ExtractBoundedSubsequence();
-        ExtractBoundedSubsequenceLength(kvlist.keys, boundaries, i);
-        Keys.IsStrictlySortedImpliesLte(kvlist.keys, boundaries[i], boundaries[i] + j);
-      }
-      reveal_AllKeys();
-    }
+  // lemma LeavesProperties(kvlist: KVList, config: Configuration, boundaries: seq<nat>, node: Node)
+  //   requires 0 < |kvlist.keys|
+  //   requires WFKVList(kvlist)
+  //   requires ValidConfiguration(config)
+  //   requires boundaries == BuildBoundaries(|kvlist.keys|, config.maxKeys)
+  //   requires node.Index?
+  //   requires node.children == BuildLeavesForSequence(kvlist, boundaries)
+  //   requires node.pivots == ExtractPivotsForBoundaries(ExtractPivotsFromKVList(kvlist), boundaries)
+  //   ensures WF(node)
+  //   ensures Interpretation(node) == KVListInterpretation(kvlist)
+  //   ensures forall i :: 0 <= i < |node.children| ==> FitsConfig(node.children[i], config)
+  // {
+  //   ExtractPivotsForBoundariesPreservesSort(ExtractPivotsFromKVList(kvlist), boundaries);
+  //   reveal_ExtractPivotsForBoundaries();
+  //   forall i | 0 <= i < |node.children| - 1
+  //     ensures AllKeysBelowBound(node, i)
+  //   {
+  //     forall j | 0 <= j < |node.children[i].keys|
+  //       ensures Keys.lt(node.children[i].keys[j], node.pivots[i])
+  //     {
+  //       reveal_ExtractBoundedSubsequence();
+  //       ExtractBoundedSubsequenceLength(kvlist.keys, boundaries, i);
+  //       Keys.IsStrictlySortedImpliesLt(kvlist.keys, boundaries[i] + j, boundaries[i+1]);
+  //     }
+  //     reveal_AllKeys();
+  //   }
+  //   forall i | 0 < i < |node.children|
+  //     ensures AllKeysAboveBound(node, i)
+  //   {
+  //     forall j | 0 <= j < |node.children[i].keys|
+  //       ensures Keys.lte(node.pivots[i-1], node.children[i].keys[j])
+  //     {
+  //       reveal_ExtractBoundedSubsequence();
+  //       ExtractBoundedSubsequenceLength(kvlist.keys, boundaries, i);
+  //       Keys.IsStrictlySortedImpliesLte(kvlist.keys, boundaries[i], boundaries[i] + j);
+  //     }
+  //     reveal_AllKeys();
+  //   }
 
-    forall i | 0 <= i < |node.children|
-      ensures FitsConfig(node.children[i], config)
-    {
-      ExtractBoundedSubsequenceLength(kvlist.keys, boundaries, i);
-      reveal_BoundariesFit();
-    }
+  //   forall i | 0 <= i < |node.children|
+  //     ensures FitsConfig(node.children[i], config)
+  //   {
+  //     ExtractBoundedSubsequenceLength(kvlist.keys, boundaries, i);
+  //     reveal_BoundariesFit();
+  //   }
     
-    var inode := Interpretation(node);
-    var ikvlist := KVListInterpretation(kvlist);
+  //   var inode := Interpretation(node);
+  //   var ikvlist := KVListInterpretation(kvlist);
     
-    forall k | k in inode
-      ensures MapsTo(ikvlist, k, inode[k])
-    {
-      reveal_ExtractBoundedSubsequence();
-      var childidx := Keys.LargestLte(node.pivots, k) + 1;
-      var child := node.children[childidx];
-      InterpretationInheritance(node, k);
-      assert k in child.keys by { reveal_Interpretation(); }
-      var j := Keys.LargestLte(child.keys, k);
-      Keys.PosEqLargestLte(kvlist.keys, k, boundaries[childidx] + j);
-      assert child.values[j] == inode[k] by { reveal_Interpretation(); }
-    }
+  //   forall k | k in inode
+  //     ensures MapsTo(ikvlist, k, inode[k])
+  //   {
+  //     reveal_ExtractBoundedSubsequence();
+  //     var childidx := Keys.LargestLte(node.pivots, k) + 1;
+  //     var child := node.children[childidx];
+  //     InterpretationInheritance(node, k);
+  //     assert k in child.keys by { reveal_Interpretation(); }
+  //     var j := Keys.LargestLte(child.keys, k);
+  //     Keys.PosEqLargestLte(kvlist.keys, k, boundaries[childidx] + j);
+  //     assert child.values[j] == inode[k] by { reveal_Interpretation(); }
+  //   }
 
-    forall k | k in ikvlist
-      ensures k in inode
-    {
-      reveal_ExtractBoundedSubsequence();
-      var pos := Keys.LargestLte(kvlist.keys, k);
-      assert 0 <= pos;
-      var childidx := Integer_Order.LargestLte(boundaries, pos);
-      assert 0 <= childidx;
-      var j := pos - boundaries[childidx];
-      if 0 <= childidx - 1 {
-      }
-      if childidx - 1 < |node.pivots|-1 {
-      }
-      Keys.LargestLteIsUnique2(node.pivots, k, childidx-1);
-      assert childidx-1 == Keys.LargestLte(node.pivots, k);
-      var child := node.children[childidx];
-      assert child.keys[j] == k;
-      assert k in Interpretation(child) by { reveal_Interpretation(); }
-      InterpretationDelegation(node, k);
-    }
+  //   forall k | k in ikvlist
+  //     ensures k in inode
+  //   {
+  //     reveal_ExtractBoundedSubsequence();
+  //     var pos := Keys.LargestLte(kvlist.keys, k);
+  //     assert 0 <= pos;
+  //     var childidx := Integer_Order.LargestLte(boundaries, pos);
+  //     assert 0 <= childidx;
+  //     var j := pos - boundaries[childidx];
+  //     if 0 <= childidx - 1 {
+  //     }
+  //     if childidx - 1 < |node.pivots|-1 {
+  //     }
+  //     Keys.LargestLteIsUnique2(node.pivots, k, childidx-1);
+  //     assert childidx-1 == Keys.LargestLte(node.pivots, k);
+  //     var child := node.children[childidx];
+  //     assert child.keys[j] == k;
+  //     assert k in Interpretation(child) by { reveal_Interpretation(); }
+  //     InterpretationDelegation(node, k);
+  //   }
     
-  }
+  // }
   
-  function BuildTreeForSequence(kvlist: KVList, config: Configuration) : (node: Node)
-    requires 0 < |kvlist.keys|
-    requires WFKVList(kvlist)
-    requires ValidConfiguration(config)
-    ensures FitsConfig(node, config)
-    ensures Interpretation(node) == KVListInterpretation(kvlist)
-  {
-    var boundaries := BuildBoundaries(|kvlist.keys|, config.maxKeys);
-    var leaves := BuildLeavesForSequence(kvlist, boundaries);
-    var pivots := ExtractPivotsForBoundaries(ExtractPivotsFromKVList(kvlist), boundaries);
-    var node := Index(pivots, leaves);
-    LeavesProperties(kvlist, config, boundaries, node);
-    BuildLayers(leaves, pivots, config)
-  }
+  // function BuildTreeForSequence(kvlist: KVList, config: Configuration) : (node: Node)
+  //   requires 0 < |kvlist.keys|
+  //   requires WFKVList(kvlist)
+  //   requires ValidConfiguration(config)
+  //   ensures FitsConfig(node, config)
+  //   ensures Interpretation(node) == KVListInterpretation(kvlist)
+  // {
+  //   var boundaries := BuildBoundaries(|kvlist.keys|, config.maxKeys);
+  //   var leaves := BuildLeavesForSequence(kvlist, boundaries);
+  //   var pivots := ExtractPivotsForBoundaries(ExtractPivotsFromKVList(kvlist), boundaries);
+  //   var node := Index(pivots, leaves);
+  //   LeavesProperties(kvlist, config, boundaries, node);
+  //   BuildLayers(leaves, pivots, config)
+  // }
 }
 
